@prefix marl:     <http://purl.org/marl/ns#>.
@prefix nif:      <http://persistence.uni-leipzig.org/nlp2rdf/ontologies/nif-core#>.

# NOTE1: is this a good namespace for our own properties
@prefix ms:       <http://data.multisensor.eu/ontology#>.

# NOTE2: Multisensor ontology. This will be stated only once, NOT with every sentence

ms:negativePolarityValue a owl:DatatypeProperty;
  rdfs:domain marl:Opinion;
  rdfs:label "Negative polarity value"@en;
  rdfs:comment "A sentence may include both negative and positive polarity words"@en;
  rdfs:isDefinedBy <http://data.multisensor.eu/ontology>.

ms:positivePolarityValue a owl:DatatypeProperty;
  rdfs:domain marl:Opinion;
  rdfs:label "Positive polarity value"@en;
  rdfs:comment "A sentence may include both negative and positive polarity words"@en;
  rdfs:isDefinedBy <http://data.multisensor.eu/ontology>.

ms:sentimentalityValue a owl:DatatypeProperty;
  rdfs:domain marl:Opinion;
  rdfs:label "Sentimentality value"@en;
  rdfs:comment "Difference between the positive and negative polarity of an opinion (eg a sentence)"@en;
  rdfs:isDefinedBy <http://data.multisensor.eu/ontology>.

# NOTE3: Sentences are already demarkated by another MS partner
<http://data.multisensor.eu/content/guid#char=100,200> a nif:Sentence.

# Sentiment
<http://data.multisensor.eu/content/guid#char=100,200>
  nif:opinion <http://data.multisensor.eu/content/guid#char=100,200-sentiment>.
<http://data.multisensor.eu/content/guid#char=100,200-sentiment>
  a marl:Opinion;
  marl:minPolarityValue    -5.0;
  marl:maxPolarityValue     5.0;
  ms:negativePolarityValue -3.5;
  ms:positivePolarityValue  2.0;
  marl:polarityValue       -1.5;
  ms:sentimentalityValue    5.5.

# NOTE4: Maybe marl:polarityValue should be the AVERAGE of pos and neg not the SUM?
