@base <http://data.multisensorproject.eu/content/53a0938bc4770c6ba0e7d7b9ca88a637f9e9c304>.
@prefix marl:     <http://purl.org/marl/ns#>.
@prefix nif:      <http://persistence.uni-leipzig.org/nlp2rdf/ontologies/nif-core#>.

# NOTE1: namespace for our own properties
@prefix ms:       <http://data.multisensorproject.eu/ontology#>.

# NOTE2: Multisensor ontology. This will be stated only once, NOT with every sentence

ms:negativePolarityValue a owl:DatatypeProperty;
  rdfs:domain marl:Opinion;
  rdfs:label "Most negative polarity value"@en;
  rdfs:comment "A sentence may include both negative and positive polarity words: this records the most negative polarity"@en;
  rdfs:isDefinedBy <http://data.multisensorproject.eu/ontology>.

ms:positivePolarityValue a owl:DatatypeProperty;
  rdfs:domain marl:Opinion;
  rdfs:label "Most positive polarity value"@en;
  rdfs:comment "A sentence may include both negative and positive polarity words: this records the most positive polarity"@en;
  rdfs:isDefinedBy <http://data.multisensorproject.eu/ontology>.

ms:sentimentalityValue a owl:DatatypeProperty;
  rdfs:domain marl:Opinion;
  rdfs:label "Sentimentality value"@en;
  rdfs:comment "Difference between the most positive and most negative polarity of an opinion (eg a sentence)"@en;
  rdfs:isDefinedBy <http://data.multisensorproject.eu/ontology>.

marl:polarityValue  rdfs:comment "This is the AVERAGE of ALL pos and neg opinions, not the SUM of ONLY the extremal opinions"@en.

# NOTE3: Sentences and the context are already demarkated by another MS partner
<http://data.multisensorproject.eu/content/53a0938bc4770c6ba0e7d7b9ca88a637f9e9c304#char=0,2000> a nif:Context;
  nif:isString "This is the whole text of the SIMMO. It should continue for 2000 chars but I'll stop here"@en.
<http://data.multisensorproject.eu/content/53a0938bc4770c6ba0e7d7b9ca88a637f9e9c304#char=100,200> a nif:Sentence;
  nif:referenceContext <http://data.multisensorproject.eu/content/53a0938bc4770c6ba0e7d7b9ca88a637f9e9c304#char=0,2000>.

# Sentiment of the whole news item (SIMMO)
<http://data.multisensorproject.eu/content/53a0938bc4770c6ba0e7d7b9ca88a637f9e9c304#char=0,2000>
  nif:opinion <http://data.multisensorproject.eu/content/53a0938bc4770c6ba0e7d7b9ca88a637f9e9c304#char=0,2000-sentiment>.
<http://data.multisensorproject.eu/content/53a0938bc4770c6ba0e7d7b9ca88a637f9e9c304#char=100,200-sentiment>
  a marl:Opinion;
  marl:minPolarityValue    -5.0; # sentiment range: minimum
  marl:maxPolarityValue     5.0; # sentiment range: maximum
  ms:negativePolarityValue -3.5; # most negative sentiment
  ms:positivePolarityValue  2.0; # most positive sentiment
  marl:polarityValue       -1.5; # sum of the two polar opinions (what's the average sentiment)
  ms:sentimentalityValue    5.5. # difference of the two polar opinions (how strong is the sentiment)

# Sentiment of a sentence. Structured exactly as above
<http://data.multisensorproject.eu/content/53a0938bc4770c6ba0e7d7b9ca88a637f9e9c304#char=100,200>
  nif:opinion <http://data.multisensorproject.eu/content/53a0938bc4770c6ba0e7d7b9ca88a637f9e9c304#char=100,200-sentiment>.

<http://data.multisensorproject.eu/content/53a0938bc4770c6ba0e7d7b9ca88a637f9e9c304#char=100,200-sentiment>
  a marl:Opinion;
  marl:minPolarityValue    -5.0;
  marl:maxPolarityValue     5.0;
  ms:negativePolarityValue -3.5;
  ms:positivePolarityValue  2.0;
  marl:polarityValue       -1.5;
  ms:sentimentalityValue    5.5.

# Sentence without any sentiment-bearing words.

<http://data.multisensorproject.eu/content/53a0938bc4770c6ba0e7d7b9ca88a637f9e9c304#char=200,300>
  a <http://data.multisensorproject.eu/content/53a0938bc4770c6ba0e7d7b9ca88a637f9e9c304#char=200,300-sentiment>.
  
<http://data.multisensorproject.eu/content/53a0938bc4770c6ba0e7d7b9ca88a637f9e9c304#char=200,300-sentiment>
  a marl:Opinion;
  marl:minPolarityValue    -5.0;
  marl:maxPolarityValue     5.0;
  # ms:negativePolarityValue & ms:positivePolarityValue & marl:polarityValue are omitted
  ms:sentimentalityValue    0.0.
